IMLTT/typed/proofs/Recursor.lean
@@ -40,8 +40,8 @@ theorem judgment_recursor :
   → (HasTypePiIntro : ∀ {n : Nat} {Γ : Ctx n} {A : Tm n} {b B : Tm (n + 1)} 
     (a : (Γ ⬝ A) ⊢ b ∶ B), motive_3 (Γ ⬝ A) b B a → motive_3 Γ (.lam A b) (.pi A B) (HasType.pi_intro a))
   → (HasTypeSigmaIntro : ∀ {n : Nat} {Γ : Ctx n} {a A b : Tm n} {B : Tm (n + 1)} 
-    (a_1 : Γ ⊢ a ∶ A) (a_2 : Γ ⊢ b ∶ substitute_zero B a),
-    motive_3 Γ a A a_1 → motive_3 Γ b (substitute_zero B a) a_2
+    (a_1 : Γ ⊢ a ∶ A) (a_2 : Γ ⊢ b ∶ substitute_zero a B),
+    motive_3 Γ a A a_1 → motive_3 Γ b (substitute_zero a B) a_2
     → motive_3 Γ (.pairSigma a b) (.sigma A B) (HasType.sigma_intro a_1 a_2))
   → (HasTypeIdenIntro : ∀ {n : Nat} {Γ : Ctx n} {A a : Tm n} 
     (a_2 : Γ ⊢ a ∶ A),
@@ -62,17 +62,17 @@ theorem judgment_recursor :
     motive_3 Γ A 𝒰 a_1 → motive_3 Γ a A a_2 → motive_3 Γ a' A a_3 
     → motive_3 Γ (.iden A a a') 𝒰 (HasType.univ_iden a_1 a_2 a_3))
   → (HasTypeUnitElim : ∀ {n : Nat} {Γ : Ctx n} {A : Tm (n + 1)} {a b : Tm n} 
-    (a_1 : (Γ ⬝ 𝟙) ⊢ A type) (a_2 : Γ ⊢ a ∶ substitute_zero A ⋆) (a_3 : Γ ⊢ b ∶ 𝟙),
-    motive_2 (Γ ⬝ 𝟙) A a_1 → motive_3 Γ a (substitute_zero A ⋆) a_2 → motive_3 Γ b 𝟙 a_3 
-    → motive_3 Γ (.indUnit A b a) (substitute_zero A b) (HasType.unit_elim a_1 a_2 a_3))
+    (a_1 : (Γ ⬝ 𝟙) ⊢ A type) (a_2 : Γ ⊢ a ∶ substitute_zero ⋆ A) (a_3 : Γ ⊢ b ∶ 𝟙),
+    motive_2 (Γ ⬝ 𝟙) A a_1 → motive_3 Γ a (substitute_zero ⋆ A) a_2 → motive_3 Γ b 𝟙 a_3 
+    → motive_3 Γ (.indUnit A b a) (substitute_zero b A) (HasType.unit_elim a_1 a_2 a_3))
   → (HasTypeEmptyElim : ∀ {n : Nat} {Γ : Ctx n} {A : Tm (n + 1)} {b : Tm n} 
     (a : (Γ ⬝ 𝟘) ⊢ A type) (a_1 : Γ ⊢ b ∶ 𝟘), 
     motive_2 (Γ ⬝ 𝟘) A a → motive_3 Γ b 𝟘 a_1 
-    → motive_3 Γ (.indEmpty A b) (substitute_zero A b) (HasType.empty_elim a a_1))
+    → motive_3 Γ (.indEmpty A b) (substitute_zero b A) (HasType.empty_elim a a_1))
   → (HasTypePiElim : ∀ {n : Nat} {Γ : Ctx n} {f A : Tm n} {B : Tm (n + 1)} {a : Tm n} 
     (a_1 : Γ ⊢ f ∶ (.pi A B)) (a_2 : Γ ⊢ a ∶ A),
     motive_3 Γ f (.pi A B) a_1 → motive_3 Γ a A a_2 
-    → motive_3 Γ (.app f a) (substitute_zero B a) (HasType.pi_elim a_1 a_2))
+    → motive_3 Γ (.app f a) (substitute_zero a B) (HasType.pi_elim a_1 a_2))
   → (HasTypeSigmaElim : ∀ {n : Nat} {Γ : Ctx n} {A : Tm n} {B : Tm (n + 1)} {p : Tm n} 
     {C : Tm (n + 1)} {c : Tm (n + 1 + 1)}
     (a_1 : Γ ⊢ p ∶ (.sigma A B)) (a_2 : (Γ ⬝ (.sigma A B)) ⊢ C type)
@@ -81,7 +81,7 @@ theorem judgment_recursor :
     motive_3 Γ p (.sigma A B) a_1 → motive_2 (Γ ⬝ (.sigma A B)) C a_2
     → motive_3 (Γ ⬝ A ⬝ B) c
       (substitute (Subst.weak (.shift (.shift .id)), (.pairSigma v(1) v(0))) C) a_3
-    → motive_3 Γ (.indSigma A B C c p) (substitute_zero C p) (HasType.sigma_elim a_1 a_2 a_3) )
+    → motive_3 Γ (.indSigma A B C c p) (substitute_zero p C) (HasType.sigma_elim a_1 a_2 a_3) )
   → (HasTypeIdenElim : ∀ {n : Nat} {Γ : Ctx n} {A : Tm n} {B : Tm (n + 1 + 1 + 1)} {b : Tm n} 
     {a a' p : Tm n}
     (a_1 : (Γ ⬝ A ⬝ (weaken Weak.id.shift A) ⬝ (weaken Weak.id.shift.shift A).iden v(1) v(0)) ⊢ B type)
@@ -120,21 +120,21 @@ theorem judgment_recursor :
     (a : Γ ⊢ A type), motive_2 Γ A a 
     → motive_5 (Γ ⬝ A) v(0) v(0) (weaken Weak.id.shift A) (IsEqualTerm.var_eq a))
   → (IsEqualTermUnitComp : ∀ {n : Nat} {Γ : Ctx n} {A : Tm (n + 1)} {a : Tm n} 
-    (a_1 : (Γ ⬝ 𝟙) ⊢ A type) (a_2 : Γ ⊢ a ∶ substitute_zero A ⋆),
-    motive_2 (Γ ⬝ 𝟙) A a_1 → motive_3 Γ a (substitute_zero A ⋆) a_2 
-    → motive_5 Γ (A.indUnit ⋆ a) a (substitute_zero A ⋆) (IsEqualTerm.unit_comp a_1 a_2))
+    (a_1 : (Γ ⬝ 𝟙) ⊢ A type) (a_2 : Γ ⊢ a ∶ substitute_zero ⋆ A),
+    motive_2 (Γ ⬝ 𝟙) A a_1 → motive_3 Γ a (substitute_zero ⋆ A) a_2 
+    → motive_5 Γ (A.indUnit ⋆ a) a (substitute_zero ⋆ A) (IsEqualTerm.unit_comp a_1 a_2))
   → (IsEqualTermPiComp : ∀ {n : Nat} {Γ : Ctx n} {A : Tm n} {b B : Tm (n + 1)} {a : Tm n} 
     (a_1 : (Γ ⬝ A) ⊢ b ∶ B) (a_2 : Γ ⊢ a ∶ A), motive_3 (Γ ⬝ A) b B a_1 → motive_3 Γ a A a_2 
-    → motive_5 Γ ((A.lam b).app a) (substitute_zero b a) (substitute_zero B a) 
+    → motive_5 Γ ((A.lam b).app a) (substitute_zero a b) (substitute_zero a B) 
       (IsEqualTerm.pi_comp a_1 a_2))
   → (IsEqualTermSigmaComp : ∀ {n : Nat} {Γ : Ctx n} {a A b : Tm n} {B C : Tm (n + 1)} 
     {c : Tm (n + 1 + 1)} (a_1 : Γ ⊢ a ∶ A)
-    (a_2 : Γ ⊢ b ∶ substitute_zero B a) (a_3 : (Γ ⬝ A.sigma B) ⊢ C type)
+    (a_2 : Γ ⊢ b ∶ substitute_zero a B) (a_3 : (Γ ⬝ A.sigma B) ⊢ C type)
     (a_4 : (Γ ⬝ A ⬝ B) ⊢ c ∶ substitute (Subst.weak Weak.id.shift.shift, v(1).pairSigma v(0)) C),
-    motive_3 Γ a A a_1 → motive_3 Γ b (substitute_zero B a) a_2 → motive_2 (Γ ⬝ A.sigma B) C a_3 
+    motive_3 Γ a A a_1 → motive_3 Γ b (substitute_zero a B) a_2 → motive_2 (Γ ⬝ A.sigma B) C a_3 
     → motive_3 (Γ ⬝ A ⬝ B) c (substitute (Subst.weak Weak.id.shift.shift, v(1).pairSigma v(0)) C) a_4 
     → motive_5 Γ (A.indSigma B C c (a.pairSigma b)) (substitute (Subst.weak Weak.id, a, b) c)
-      (substitute_zero C (a.pairSigma b)) (IsEqualTerm.sigma_comp a_1 a_2 a_3 a_4))
+      (substitute_zero (a.pairSigma b) C) (IsEqualTerm.sigma_comp a_1 a_2 a_3 a_4))
   → (IsEqualTermIdenComp : ∀ {n : Nat} {Γ : Ctx n} {A : Tm n} {B : Tm (n + 1 + 1 + 1)} 
     {b : Tm n} {a : Tm n}
     (a_1 : (Γ ⬝ A ⬝ (weaken Weak.id.shift A) ⬝ (weaken Weak.id.shift.shift A).iden v(1) v(0)) ⊢ B type)
@@ -148,23 +148,23 @@ theorem judgment_recursor :
   → (IsEqualTermUnitIntroEq : ∀ {n : Nat} {Γ : Ctx n} 
     (a : Γ ctx), motive_1 Γ a → motive_5 Γ ⋆ ⋆ 𝟙 (IsEqualTerm.unit_intro_eq a))
   → (IsEqualTermUnitElimEq : ∀ {n : Nat} {Γ : Ctx n} {A A' : Tm (n + 1)} {a a' b b' : Tm n} 
-    (a_1 : (Γ ⬝ 𝟙) ⊢ A ≡ A' type) (a_2 : Γ ⊢ a ≡ a' ∶ substitute_zero A ⋆) (a_3 : Γ ⊢ b ≡ b' ∶ 𝟙),
-    motive_4 (Γ ⬝ 𝟙) A A' a_1 → motive_5 Γ a a' (substitute_zero A ⋆) a_2 → motive_5 Γ b b' 𝟙 a_3 
-    → motive_5 Γ (A.indUnit b a) (A'.indUnit b' a') (substitute_zero A b) 
+    (a_1 : (Γ ⬝ 𝟙) ⊢ A ≡ A' type) (a_2 : Γ ⊢ a ≡ a' ∶ substitute_zero ⋆ A) (a_3 : Γ ⊢ b ≡ b' ∶ 𝟙),
+    motive_4 (Γ ⬝ 𝟙) A A' a_1 → motive_5 Γ a a' (substitute_zero ⋆ A) a_2 → motive_5 Γ b b' 𝟙 a_3 
+    → motive_5 Γ (A.indUnit b a) (A'.indUnit b' a') (substitute_zero b A) 
       (IsEqualTerm.unit_elim_eq a_1 a_2 a_3))
   → (IsEqualTermEmptyElimEq : ∀ {n : Nat} {Γ : Ctx n} {A A' : Tm (n + 1)} {b b' : Tm n} 
     (a : (Γ ⬝ 𝟘) ⊢ A ≡ A' type) (a_1 : Γ ⊢ b ≡ b' ∶ 𝟘), motive_4 (Γ ⬝ 𝟘) A A' a → motive_5 Γ b b' 𝟘 a_1 
-    → motive_5 Γ (A.indEmpty b) (A'.indEmpty b') (substitute_zero A b) (IsEqualTerm.empty_elim_eq a a_1))
+    → motive_5 Γ (A.indEmpty b) (A'.indEmpty b') (substitute_zero b A) (IsEqualTerm.empty_elim_eq a a_1))
   → (IsEqualTermPiIntroEq : ∀ {n : Nat} {Γ : Ctx n} {A : Tm n} {b b' B : Tm (n + 1)} {A' : Tm n} 
     (a : (Γ ⬝ A) ⊢ b ≡ b' ∶ B), motive_5 (Γ ⬝ A) b b' B a 
     → motive_5 Γ (A.lam b) (A'.lam b') (A.pi B) (IsEqualTerm.pi_intro_eq a))
   → (IsEqualTermPiElimEq : ∀ {n : Nat} {Γ : Ctx n} {f f' A : Tm n} {B : Tm (n + 1)} {a a' : Tm n} 
     (a_1 : Γ ⊢ f ≡ f' ∶ A.pi B) (a_2 : Γ ⊢ a ≡ a' ∶ A), motive_5 Γ f f' (A.pi B) a_1 
-    → motive_5 Γ a a' A a_2 → motive_5 Γ (f.app a) (f'.app a') (substitute_zero B a) 
+    → motive_5 Γ a a' A a_2 → motive_5 Γ (f.app a) (f'.app a') (substitute_zero a B) 
       (IsEqualTerm.pi_elim_eq a_1 a_2))
   → (IsEqualTermSigmaIntroEq : ∀ {n : Nat} {Γ : Ctx n} {a a' A b b' : Tm n} {B : Tm (n + 1)} 
-    (a_1 : Γ ⊢ a ≡ a' ∶ A) (a_2 : Γ ⊢ b ≡ b' ∶ substitute_zero B a), motive_5 Γ a a' A a_1 
-    → motive_5 Γ b b' (substitute_zero B a) a_2 
+    (a_1 : Γ ⊢ a ≡ a' ∶ A) (a_2 : Γ ⊢ b ≡ b' ∶ substitute_zero a B), motive_5 Γ a a' A a_1 
+    → motive_5 Γ b b' (substitute_zero a B) a_2 
     → motive_5 Γ (a.pairSigma b) (a'.pairSigma b') (A.sigma B) (IsEqualTerm.sigma_intro_eq a_1 a_2))
   → (IsEqualTermSigmaElimEq :  ∀ {n : Nat} {Γ : Ctx n} {A : Tm n} {B : Tm (n + 1)} {A' : Tm n} 
     {B' : Tm (n + 1)} {p p' : Tm n} {C C' : Tm (n + 1)} {c c' : Tm (n + 1 + 1)} 
@@ -174,7 +174,7 @@ theorem judgment_recursor :
     motive_4 Γ (A.sigma B) (A'.sigma B') a → motive_5 Γ p p' (A.sigma B) a_1 
     → motive_4 (Γ ⬝ A.sigma B) C C' a_2 
     → motive_5 (Γ ⬝ A ⬝ B) c c' (substitute (Subst.weak Weak.id.shift.shift, v(1).pairSigma v(0)) C) a_3
-    → motive_5 Γ (A.indSigma B C c p) (A'.indSigma B' C' c' p') (substitute_zero C p)
+    → motive_5 Γ (A.indSigma B C c p) (A'.indSigma B' C' c' p') (substitute_zero p C)
       (IsEqualTerm.sigma_elim_eq a a_1 a_2 a_3))
   → (IsEqualTermIdenIntroEq : ∀ {n : Nat} {Γ : Ctx n} {A A' a a' : Tm n} 
     (a_1 : Γ ⊢ A ≡ A' type) (a_2 : Γ ⊢ a ≡ a' ∶ A), motive_4 Γ A A' a_1 → motive_5 Γ a a' A a_2 
